coq/dec_implicit/Dec.v
@@ -3,6 +3,8 @@ Require Import Algo.
 Require Import Lia.
 From Hammer Require Import Tactics.
 Require Import Coq.Program.Equality.
+Require Import Coq.Arith.Compare_dec.
+Require Import Coq.Arith.PeanoNat.
 
 Fixpoint tm_size (e : Trm) : nat :=
   match e with
@@ -35,9 +37,326 @@ Lemma dec_CtxEmpty Σ :
   {Σ = CtxEmpty} + {NonEmpty Σ}.
 Proof. sauto lq: on. Qed.
 
-Lemma dec_sub : forall Δ A p B,
+Lemma eq_dec_ty : forall (A B : Typ),
+  {A = B} + {A <> B}.
+Proof.  decide equality. decide equality. Qed.
+
+Lemma dec_ty_unshift : forall A k,
+  {A' | A = ty_shift A' k} + {~ exists A', A = ty_shift A' k}.
+Proof.
+  intro A; induction A; intro k.
+  - left. exists Int. sfirstorder.
+  - destruct (lt_dec n k) as [Hlt | Hlt].
+    + left. exists (TVar n). simpl. unfold punchIn. sauto l: on.
+    + assert (Hle: k <= n) by lia.
+      destruct n.
+      * right. intros [A' Heq].
+        destruct A'; try sfirstorder.
+        sauto q: on.
+      * destruct (le_dec k n) as [Hle' | Hle'].
+        -- left. exists (TVar n). simpl. unfold punchIn. sauto l: on.
+        -- assert (Heq: k = S n) by lia. subst. 
+           right. intros [A' Heq].
+           destruct A'; try sfirstorder.
+           dependent destruction Heq. unfold punchIn in *.
+           destruct (Nat.leb (S n) n0) eqn:Hle''; unfold punchIn in *; hauto lqb: on.
+  - specialize (IHA1 k). specialize (IHA2 k).
+    destruct IHA1 as [[A1' Heq1] | Hneq1]; destruct IHA2 as [[A2' Heq2] | Hneq2]; subst.
+    + left. exists (Arr A1' A2'). sfirstorder.
+    + right. intros [A' Heq]. destruct A'; try sfirstorder.
+    + right. intros [A' Heq]. destruct A'; try sfirstorder.
+    + right. intros [A' Heq]. destruct A'; try sfirstorder.
+  - specialize (IHA (S k)). destruct IHA as [[A' Heq] | Hneq]; subst.
+    + left. exists (All A'). sfirstorder.
+    + right. intros [A'' Heq]. destruct A''; try sfirstorder.
+Qed.
+
+Lemma ty_unshift_det : forall B k A1 A2,
+  B = ty_shift A1 k -> B = ty_shift A2 k -> A1 = A2.
+Proof.
+  intro B. induction B; intros k A1 A2 Heq1 Heq2;
+    destruct A1; destruct A2; try sfirstorder; simpl in *.
+  - unfold punchIn in *.
+    destruct (le_dec k n0); destruct (le_dec k n1).
+    sauto l: on. hauto l: on. sauto lq: on. hauto q: on.
+  - hauto lq: on rew: off.
+  - hauto q: on.
+Qed.
+
+(* Lemma lookupTm : forall Γ x,
+  {A | lookupTm Γ x A} + {~ exists A, lookupTm Γ x A}.
+Proof.
+  intro Γ. induction Γ; intro x.
+  best.  *)
+
+Lemma dec_lookupTy : forall Γ x,
+  {lookupTy Γ x} + {~ lookupTy Γ x}.
+Proof.
+  intro Γ. induction Γ; intro x.
+  - sauto lq: on.
+  - specialize (IHΓ x). sauto lq: on.
+  - destruct x; try specialize (IHΓ x); sauto lq: on.
+  - destruct x; try specialize (IHΓ x); sauto lq: on.
+  - destruct x; try specialize (IHΓ x); sauto lq: on.
+  - specialize (IHΓ x). sauto lq: on.
+Qed.
+
+Lemma dec_lookupEx : forall Δ x,
+  {lookupEx Δ x} + {~ lookupEx Δ x}.
+Proof.
+  intro Δ. induction Δ; intro x.
+  - sauto lq: on.
+  - specialize (IHΔ x). sauto lq: on.
+  - destruct x; try specialize (IHΔ x); sauto lq: on.
+  - destruct x; try specialize (IHΔ x); sauto lq: on.
+  - destruct x; try specialize (IHΔ x); sauto lq: on.
+  - specialize (IHΔ x). sauto lq: on.
+Qed.
+
+Lemma dec_lookupExTyO : forall Δ x A,
+  {lookupExTy Δ x A} + {~ lookupExTy Δ x A}.
+Proof.
+  intro Δ. induction Δ; intros x A.
+  - sauto lq: on.
+  - destruct (dec_ty_unshift A 0) as [[A' Heq] | Hneq]; subst.
+    + specialize (IHΔ x A'). sauto q: on use: ty_unshift_det.
+    + sauto lq: on.
+  - destruct x. sauto lq: on.
+    destruct (dec_ty_unshift A 0) as [[A' Heq] | Hneq]; subst.
+    + specialize (IHΔ x A'). sauto q: on use: ty_unshift_det.
+    + sauto lq: on.
+  - destruct x. sauto lq: on.
+    destruct (dec_ty_unshift A 0) as [[A' Heq] | Hneq]; subst.
+    + specialize (IHΔ x A'). sauto q: on use: ty_unshift_det.
+    + sauto lq: on.
+  - destruct x.
+    destruct (eq_dec_ty A (ty_shift t 0)); subst; sauto lq: on.
+    destruct (dec_ty_unshift A 0) as [[A' Heq] | Hneq]; subst.
+    + specialize (IHΔ x A'). sauto q: on use: ty_unshift_det.
+    + sauto lq: on.
+  - sauto lq: on.
+Qed.
+
+Lemma dec_lookupExTy : forall Δ x,
+  {A | lookupExTy Δ x A} + {~ exists A, lookupExTy Δ x A}.
+Proof.
+  intro Δ. induction Δ; intros x.
+  - sauto lq: on.
+  - destruct (IHΔ x) as [[A' Heq] | Hneq]; sauto lq: on.
+  - destruct x. sauto lq: on.
+    destruct (IHΔ x) as [[A' Heq] | Hneq]; sauto lq: on.
+  - destruct x. sauto lq: on.
+    destruct (IHΔ x) as [[A' Heq] | Hneq]; sauto lq: on.
+  - destruct x. sauto lq: on.
+    destruct (IHΔ x) as [[A' Heq] | Hneq]; sauto lq: on.
+  - destruct x. sauto lq: on.
+    destruct (IHΔ x) as [[A' Heq] | Hneq]; sauto lq: on.
+Qed.
+
+Lemma dec_RegularTyp : forall Γ A,
+  {RegularTyp Γ A} + {~ RegularTyp Γ A}.
+Proof.
+  intros Γ A. generalize dependent Γ.
+  induction A; intro Γ; try sfirstorder.
+  - destruct (dec_lookupTy Γ n); sauto lq: on.
+  - specialize (IHA1 Γ). specialize (IHA2 Γ). sauto q: on.
+  - specialize (IHA (TyCons Γ)). sauto q: on.
+Qed.
+
+Lemma dec_Regular : forall Γ,
+  {Regular Γ} + {~ Regular Γ}.
+Proof.
+  intro Γ. induction Γ; try sfirstorder.
+  - destruct (dec_RegularTyp Γ t); sauto lq: on.
+  - sauto lq: on.
+  - sauto lq: on.
+  - destruct (dec_RegularTyp Γ t); sauto lq: on.
+  - sauto lq: on.
+Qed.
+
+Lemma dec_TRegular : forall Δ,
+  {TRegular Δ} + {~ TRegular Δ}.
+Proof.
+  intro Δ. induction Δ; try sfirstorder.
+  - destruct (dec_RegularTyp Δ t); sauto lq: on.
+  - sauto lq: on.
+  - sauto lq: on.
+  - destruct (dec_RegularTyp Δ t); sauto lq: on.
+  - sauto lq: on.
+Qed.
+
+Lemma dec_SRegular : forall Δ,
+  {SRegular Δ} + {~ SRegular Δ}.
+Proof.
+  intro Δ. induction Δ.
+  1 - 4 : sauto lq: on.
+  - destruct (dec_RegularTyp Δ t); sauto lq: on.
+  - destruct (dec_TRegular Δ); sauto lq: on.
+Qed.
+
+Lemma dec_substEnv : forall A x Γ,
+  {Γ' | substEnv A x Γ Γ'} + {~ exists Γ', substEnv A x Γ Γ'}.
+Proof.
+  intros A x Γ. generalize dependent x. generalize dependent A.
+  induction Γ; intros A x.
+  - sauto lq: on.
+  - sauto lq: on.
+  - destruct x.
+    + destruct (dec_SRegular Γ). 2 : sauto lq: on.
+      destruct (dec_ty_unshift A 0) as [[A' Heq] | Hneq]; subst. 2 : sauto lq: on.
+      destruct (dec_RegularTyp Γ A'); sauto lq: on use: ty_unshift_det.
+    + destruct (dec_ty_unshift A 0) as [[A' Heq] | Hneq]; subst.
+      * specialize (IHΓ A' x). sauto q: on use: ty_unshift_det.
+      * sauto lq: on rew: off use: ty_unshift_det.
+  - destruct x. sauto lq: on.
+    destruct (dec_ty_unshift A 0) as [[A' Heq] | Hneq]; subst.
+    + specialize (IHΓ A' x). sauto q: on use: ty_unshift_det.
+    + sauto lq: on rew: off use: ty_unshift_det.
+  - destruct x. sauto lq: on.
+    destruct (dec_ty_unshift A 0) as [[A' Heq] | Hneq]; subst. 2 : sauto lq: on.
+    destruct (dec_RegularTyp Γ t). 2 : sauto lq: on.
+    specialize (IHΓ A' x). destruct IHΓ.
+    + sauto lq: on use: ty_unshift_det.
+    + right. intros [Γ' Heq]. sauto lq: on rew: off use: ty_unshift_det.
+  - sauto lq: on.
+Qed.
+
+
+Lemma lookupTy_Ex : forall Δ x,
+  lookupTy Δ x -> lookupEx Δ x -> False.
+Proof. intro Δ. induction Δ; intros x Hty Hex; sauto lq: on. Qed.
+
+Lemma lookupTy_ExTy : forall Δ x A,
+  lookupTy Δ x -> lookupExTy Δ x A -> False.
+Proof. intro Δ. induction Δ; intros x A Hty Hex; sauto lq: on. Qed.
+
+Lemma lookupEx_ExTy : forall Δ x A,
+  lookupEx Δ x -> lookupExTy Δ x A -> False.
+Proof. intro Δ. induction Δ; intros x A Hex Hexty; sauto lq: on. Qed.
+
+Lemma substEnv_Ex : forall Δ A x Ψ,
+  substEnv A x Δ Ψ -> lookupEx Δ x.
+Proof. intro Δ. induction Δ; intros A x Ψ Hsubst; sauto lq: on. Qed.
+
+Definition NotVar (A : Typ) : Prop :=
+  match A with
+  | Int => True
+  | TVar _ => False
+  | Arr A1 A2 => True
+  | All A' => True
+  end.
+
+Lemma substEnv_det : forall Δ A x Ψ1 Ψ2,
+  substEnv A x Δ Ψ1 -> substEnv A x Δ Ψ2 -> Ψ1 = Ψ2.
+Proof.
+  intros Δ A x Ψ1 Ψ2 Hs1 Hs2. generalize dependent Ψ2.
+  induction Hs1; intros * Hs2; sauto lq: on rew: off use: ty_unshift_det.
+Qed.
+
+Lemma sub_det : forall Δ A p B Ω1 Ω2,
+  sub Δ A p B Ω1 -> sub Δ A p B Ω2 -> Ω1 = Ω2.
+Proof.
+  intros Δ A p B Ω1 Ω2 Hsub1 Hsub2. generalize dependent Ω2.
+  induction Hsub1; intros * Hsub2;
+  sauto l: on use: lookupTy_Ex, lookupTy_ExTy, lookupEx_ExTy, substEnv_Ex, substEnv_det.
+Qed.
+
+Lemma dec_sub' : forall n Δ A p B,
+  ty_size A + ty_size B < n ->
   {Ω | sub Δ A p B Ω} + {~ exists Ω, sub Δ A p B Ω}.
-Admitted.
+Proof.
+  intro n. induction n; intros Δ A p B Hlt; try lia.
+  assert (TVarL: forall x, A = TVar x -> NotVar B -> {Ω | sub Δ A p B Ω} + {~ exists Ω, sub Δ A p B Ω}).
+  { intros x Heq Hnvar. subst.
+    destruct p. 2 : sauto lq: on.
+    destruct (dec_substEnv B x Δ) as [[Δ' Hsubst] | Hsubst]. sauto lq: on.
+    destruct (dec_SRegular Δ). 2 : sauto lq: on.
+    destruct (dec_lookupExTyO Δ x B); sauto lq: on. }
+  assert (TVarR: forall x, NotVar A -> B = TVar x -> {Ω | sub Δ A p B Ω} + {~ exists Ω, sub Δ A p B Ω}).
+  { intros x Hnvar Heq. subst.
+    destruct p. sauto lq: on.
+    destruct (dec_substEnv A x Δ) as [[Δ' Hsubst] | Hsubst]. sauto lq: on.
+    destruct (dec_SRegular Δ). 2 : sauto lq: on.
+    destruct (dec_lookupExTyO Δ x A); sauto lq: on. }
+  destruct A.
+  - destruct B.
+    + destruct (dec_SRegular Δ); sauto lq: on.
+    + hauto lq: on use: TVarR.
+    + sauto lq: on.
+    + sauto lq: on.
+  - clear TVarR. destruct B.
+    + hauto lq: on use: TVarL. 
+    + clear TVarL. destruct (dec_lookupTy Δ n0).
+      * destruct (dec_lookupTy Δ n1).
+        -- destruct (Nat.eq_dec n0 n1); subst.
+           ++ destruct (dec_SRegular Δ). sauto lq: on.
+              sauto lq: on use: lookupTy_Ex, lookupTy_ExTy, substEnv_Ex.
+           ++ sauto lq: on use: lookupTy_Ex, lookupTy_ExTy, substEnv_Ex.
+        -- destruct p. sauto lq: on use: lookupTy_Ex, lookupTy_ExTy, substEnv_Ex.
+           destruct (dec_substEnv (TVar n0) n1 Δ) as [[Δ' Hsubst] | Hsubst]. sauto lq: on.
+           destruct (dec_lookupExTyO Δ n1 (TVar n0)).
+           ++ destruct (dec_SRegular Δ). sauto lq: on.
+              sauto lq: on use: lookupTy_Ex, lookupTy_ExTy, substEnv_Ex.
+           ++ sauto lq: on use: lookupTy_Ex, lookupTy_ExTy, substEnv_Ex.
+      * destruct (dec_substEnv (TVar n1) n0 Δ) as [[Δ' Hsubst] | Hsubst].
+        -- destruct p. sauto lq: on.
+           destruct (dec_substEnv (TVar n0) n1 Δ) as [[Δ'' Hsubst'] | Hsubst']. sauto lq: on.
+           destruct (dec_SRegular Δ). 2 : sauto lq: on.
+           destruct (dec_lookupExTyO Δ n1 (TVar n0)). sauto lq: on.
+           sauto lq: on use: lookupTy_Ex, lookupTy_ExTy, substEnv_Ex.
+        -- destruct (dec_lookupExTyO Δ n0 (TVar n1)).
+           ++ destruct (dec_SRegular Δ).
+              ** destruct p. sauto lq: on use: lookupTy_Ex, lookupTy_ExTy, substEnv_Ex.
+                 destruct (dec_lookupTy Δ n1). sauto lq: on use: lookupTy_Ex, lookupTy_ExTy, substEnv_Ex.
+                 destruct (dec_substEnv (TVar n0) n1 Δ) as [[Δ' Hsubst'] | Hsubst']. sauto lq: on.
+                 destruct (dec_lookupExTyO Δ n1 (TVar n0)). sauto lq: on.
+                 sauto lq: on use: lookupTy_Ex, lookupTy_ExTy, substEnv_Ex.
+              ** destruct p. sauto lq: on.
+                 destruct (dec_lookupTy Δ n1). sauto lq: on use: lookupTy_Ex, lookupTy_ExTy, substEnv_Ex.
+                 destruct (dec_substEnv (TVar n0) n1 Δ) as [[Δ' Hsubst'] | Hsubst']. sauto lq: on.
+                 destruct (dec_lookupExTyO Δ n1 (TVar n0)). sauto lq: on.
+                 sauto lq: on use: lookupTy_Ex, lookupTy_ExTy, substEnv_Ex.
+           ++ destruct (dec_substEnv (TVar n0) n1 Δ) as [[Δ' Hsubst'] | Hsubst'].
+              destruct p; sauto lq: on.
+              destruct (dec_lookupExTyO Δ n1 (TVar n0)).
+              ** destruct p. sauto lq: on.
+                 destruct (dec_SRegular Δ). sauto lq: on.
+                 sauto lq: on use: lookupTy_Ex, lookupTy_ExTy, substEnv_Ex.
+              ** sauto lq: on use: lookupTy_Ex, lookupTy_ExTy, substEnv_Ex.
+    + hauto lq: on use: TVarL.
+    + hauto lq: on use: TVarL.
+  - destruct B.
+    + sauto lq: on.
+    + hauto lq: on use: TVarR.
+    + clear TVarL TVarR. simpl in *.
+      assert (Hlt1: ty_size B1 + ty_size A1 < n) by lia.
+      assert (Hlt2: ty_size A2 + ty_size B2 < n) by lia.
+      eapply IHn with (Δ := Δ) (p := neg p) in Hlt1 as IHn1.
+      destruct IHn1 as [[Ω Hsub1] | Hneg1].
+      * eapply IHn with (Δ := Ω) (p := p) in Hlt2 as IHn2.
+        destruct IHn2 as [[Ψ Hsub2] | Hneg2].
+        -- sauto lq: on.
+        -- right. intros [Ψ' Hc]. dependent destruction Hc.
+           eapply sub_det in Hsub1; eauto. subst. sfirstorder.
+      * sauto lq: on.
+    + sauto lq: on.
+  - destruct B.
+    + sauto lq: on.
+    + hauto lq: on use: TVarR.
+    + sauto lq: on.
+    + clear TVarL TVarR. simpl in *.
+      assert (Hlt': ty_size A + ty_size B < n) by lia.
+      eapply IHn with (Δ := TyCons Δ) (p := p) in Hlt' as IHn1.
+      destruct IHn1 as [[Ω Hsub] | Hneg].
+      * destruct Ω; try solve [right; intros [Ω' Hc]; dependent destruction Hc;
+          eapply sub_det in Hsub; eauto; subst; sfirstorder].
+        sauto lq: on.
+      * sauto lq: on.
+Qed.
+
+Theorem dec_sub : forall Δ A p B,
+  {Ω | sub Δ A p B Ω} + {~ exists Ω, sub Δ A p B Ω}.
+Proof. intros. eapply dec_sub'; eauto. Qed.
 
 Lemma dec_ty_sub_ctx' : forall n,
   (forall Γ Σ e, tm_size e + ctx_size Σ < n ->
@@ -45,3 +364,11 @@ Lemma dec_ty_sub_ctx' : forall n,
   (forall Δ A Σ, ctx_size Σ < n ->
     {Δ' : Env & {A' : Typ & sub_ctx Δ A Σ Δ' A'}} + {~ exists Δ' A', sub_ctx Δ A Σ Δ' A'}).
 Admitted.
+
+Theorem dec_ty : forall Γ Σ e,
+  {A | ty Γ Σ e A} + {~ exists A, ty Γ Σ e A}.
+Proof. hauto lq: on use: dec_ty_sub_ctx'. Qed.
+
+Theorem dec_sub_ctx : forall Δ A Σ,
+  {Δ' : Env & {A' : Typ & sub_ctx Δ A Σ Δ' A'}} + {~ exists Δ' A', sub_ctx Δ A Σ Δ' A'}.
+Proof. hauto lq: on use: dec_ty_sub_ctx'. Qed.
